coq_alt/Shared/Sema.v
@@ -1,0 +1,187 @@
+Set Implicit Arguments.
+Require Import Strings.String Strings.Ascii Lists.List Lia.
+Require Import CSC.Util.
+
+From RecordUpdate Require Import RecordSet.
+
+#[export]
+Instance nateq__Instance : HasEquality nat := {
+  eq := Nat.eqb ;
+  eqb_eq := PeanoNat.Nat.eqb_eq ;
+}.
+
+(** Possible binary operations. *)
+Variant binopsymb : Type :=
+| Badd : binopsymb
+| Bsub : binopsymb
+| Bmul : binopsymb
+| Bdiv : binopsymb
+| Bless : binopsymb
+.
+Definition binopsymb_eqb :=
+  fun (b1 b2 : binopsymb) =>
+    match b1, b2 with
+    | Badd, Badd | Bsub, Bsub | Bmul, Bmul | Bdiv, Bdiv | Bless, Bless => true
+    | _, _ => false
+    end
+.
+Lemma binopsymb_eqb_eq b1 b2 :
+  binopsymb_eqb b1 b2 = true <-> b1 = b2.
+Proof. destruct b1, b2; now cbn. Qed.
+#[export]
+Instance binopsymb__Instance : HasEquality binopsymb := {
+  eq := binopsymb_eqb ;
+  eqb_eq := binopsymb_eqb_eq ;
+}.
+
+(** Poison used to mark locations in our operational state. *)
+Inductive poison : Type :=
+| poisonless : poison
+| poisoned : poison
+.
+#[global]
+Notation "'◻'" := (poisonless).
+#[global]
+Notation "'☣'" := (poisoned).
+Definition poison_eqb :=
+  fun (ρ1 ρ2 : poison) =>
+    match ρ1, ρ2 with
+    | ◻, ◻ | ☣, ☣ => true
+    | _, _ => false
+    end
+.
+Lemma poison_eqb_eq ρ1 ρ2 :
+  poison_eqb ρ1 ρ2 = true <-> ρ1 = ρ2.
+Proof. destruct ρ1, ρ2; now cbn. Qed.
+#[export]
+Instance poisoneq__Instance : HasEquality poison := {
+  eq := poison_eqb ;
+  eqb_eq := poison_eqb_eq ;
+}.
+
+(** Context switch indicators. The paper calls these Transfer Tags *)
+Variant comms : Type :=
+| Qctxtocomp : comms
+| Qcomptoctx : comms
+| Qinternal : comms
+.
+Definition comms_eqb (q1 q2 : comms) :=
+  match q1, q2 with
+  | Qctxtocomp, Qctxtocomp => true
+  | Qcomptoctx, Qcomptoctx => true
+  | Qinternal, Qinternal => true
+  | _, _ => false
+  end
+.
+Lemma comms_eqb_eq (q1 q2 : comms) :
+  comms_eqb q1 q2 = true <-> q1 = q2.
+Proof. destruct q1, q2; now cbn. Qed.
+#[export]
+Instance commseq__Instance : HasEquality comms := {
+  eq := comms_eqb ;
+  eqb_eq := comms_eqb_eq ;
+}.
+Definition string_of_comms (q : comms) :=
+  match q with
+  | Qctxtocomp => "?"%string
+  | Qcomptoctx => "!"%string
+  | Qinternal => "∅"%string
+  end
+.
+
+(** Evaluation of binary expressions. Note that 0 means `true` in S, so `5 < 42` evals to `0`. *)
+Definition eval_binop (b : binopsymb) (n0 n1 : nat) : option nat :=
+  Some((match b with
+       | Bless => (if Nat.ltb n0 n1 then 0 else 1)
+       | Badd => (n0 + n1)
+       | Bdiv => (Nat.div n0 n1)
+       | Bsub => (n0 - n1)
+       | Bmul => (n0 * n1)
+       end))
+.
+
+(** The type used for variable names. *)
+Definition vart := string.
+Definition vareq := fun x y => (x =? y)%string.
+Definition dontcare := "_"%string.
+#[export]
+Instance varteq__Instance : HasEquality vart := {
+  eq := vareq ;
+  eqb_eq := String.eqb_eq ;
+}.
+
+(** References *)
+Inductive loc : Type :=
+| addr : nat -> loc
+.
+Definition loc_eqb :=
+  fun ℓ1 ℓ2 =>
+    match ℓ1, ℓ2 with
+    | addr n1, addr n2 => Nat.eqb n1 n2
+    end
+.
+Lemma loc_eqb_eq ℓ0 ℓ1 :
+  loc_eqb ℓ0 ℓ1 = true <-> ℓ0 = ℓ1.
+Proof.
+  destruct ℓ0 as [n0], ℓ1 as [n1]; split; intros H.
+  - cbn in H; rewrite PeanoNat.Nat.eqb_eq in H; now subst.
+  - inv H; apply PeanoNat.Nat.eqb_refl.
+Qed.
+#[export]
+Instance loceq__Instance : HasEquality loc := {
+  eq := loc_eqb ;
+  eqb_eq := loc_eqb_eq ;
+}.
+
+(** Operational state *)
+Section Heap.
+  (** Type of objects stored on heap. *)
+  Context {value : Type} {valueeq__Instance : HasEquality value}.
+
+  Definition heap := list (value).
+  Definition hNil : heap := nil.
+  Fixpoint Hgrow_aux (H : heap) (s : nat) (default : value) : heap :=
+    match s with
+    | 0 => H
+    | S n' => default :: Hgrow_aux H n' default
+    end
+  .
+  Definition Hgrow (H : heap) (s : nat) (default : value) : heap :=
+    Hgrow_aux H s default
+  .
+
+  Lemma Hget_none (H : heap) (n : nat) :
+    n >= List.length H -> List.nth_error H n = None.
+  Proof.
+    revert n; induction H; cbn; intros.
+    - destruct n; easy.
+    - destruct n; cbn; try easy. assert (n >= List.length H) by lia.
+      now specialize (IHlist n H1).
+  Qed.
+  Lemma Hget_some (H : heap) (n : nat) :
+    n < List.length H -> exists v, List.nth_error H n = Some v.
+  Proof.
+    revert n; induction H; cbn; intros.
+    - destruct n; easy.
+    - destruct n; cbn; try easy. exists a; easy.
+      assert (n < List.length H) by lia.
+      now specialize (IHlist n H1).
+  Qed.
+  Lemma Hset_none (H : heap) (n : nat) v :
+    n >= List.length H -> NoDupList.swap_nth_aux H n v = None.
+  Proof.
+    revert n; induction H; cbn; intros.
+    - now inv H.
+    - destruct n; try easy. assert (n >= List.length H) by lia.
+      specialize (IHlist n H1); now rewrite IHlist.
+  Qed.
+  Lemma Hset_some (H : heap) (n : nat) v :
+    n < List.length H -> exists H', NoDupList.swap_nth_aux H n v = Some H'.
+  Proof.
+    revert n; induction H; cbn; intros.
+    - destruct n; easy.
+    - destruct n; cbn; try easy. exists (v :: H); easy.
+      assert (n < List.length H) by lia.
+      specialize (IHlist n H1); deex. exists (a :: H'); now rewrite IHlist.
+  Qed.
+End Heap.
