coq_alt/Shared/Trace.v
@@ -1,0 +1,247 @@
+Set Implicit Arguments.
+Require Import Strings.String Lists.List Numbers.Natural.Peano.NPeano Lia Program.Equality.
+
+Require Import CSC.Util.Convenience.
+
+(** Typeclass to define trace model *)
+Class TraceParams : Type := {
+  Ev : Type ;
+  string_of_event : Ev -> string ;
+}.
+Section Trace.
+  Context {traceParams : TraceParams}.
+  (** A trace is an infinite stream of events.
+      Termination is modeled by infinitely many `None`.
+   *)
+  CoInductive trace :=
+  | TCons : option Ev -> trace -> trace
+  .
+  (** It is sufficient to look at trace prefixes for safety properties. *)
+  Definition tracepref := list Ev.
+
+  Fixpoint Tappend (As Bs : tracepref) : tracepref :=
+    match As with
+    | nil => Bs
+    | a :: As => a :: (Tappend As Bs)
+    end
+  .
+  Definition string_of_tracepref (t : tracepref) : string :=
+    let aux := fix string_of_tracepref_aux (t : tracepref) (acc : string) : string :=
+      match t with
+      | nil => acc
+      | a :: nil => String.append acc (string_of_event a)
+      | a :: As =>
+          let acc' := String.append acc (String.append (string_of_event a) (" · "%string))
+          in string_of_tracepref_aux As acc'
+      end in
+    aux t (""%string)
+  .
+  Inductive wherein : Ev -> tracepref -> nat -> Prop :=
+  | whereinIn : forall a As, wherein a (a :: As) 0
+  | whereinLook : forall a As b n, a <> b -> wherein a As n -> wherein a (b :: As) (S n)
+  .
+  Hint Constructors wherein : core.
+  Definition in_t (a : Ev) (As : tracepref) := exists (n : nat), wherein a As n.
+  Lemma wherein_nil (a : Ev) :
+    forall n, wherein a nil n -> False.
+  Proof. now induction n. Qed.
+  Lemma wherein_predecessor (a b: Ev) (As : tracepref) :
+    forall n, a <> b -> wherein a (b :: As) n -> wherein a As (pred n).
+  Proof.
+    intros.
+    inv H0. congruence. destruct As. inv H6. now cbn.
+  Qed.
+  Lemma wherein_eq (a : Ev) (As : tracepref) n m :
+    wherein a As n -> wherein a As m -> n = m.
+  Proof.
+    intros H; revert m; induction H; intros. inv H; easy.
+    destruct m. inv H1. congruence. inv H1; auto.
+  Qed.
+  Lemma wherein_equiv_wherein_cons (a b : Ev) (As : tracepref) n :
+    a <> b ->
+    wherein a As n <-> wherein a (b :: As) (n + 1).
+  Proof.
+    split.
+    - induction 1; intros. now constructor. specialize (IHwherein H). inv IHwherein; try easy.
+      constructor; trivial. rewrite Nat.add_comm. now constructor.
+    - intros H0. inv H0. rewrite Nat.add_comm in H5; congruence. rewrite Nat.add_comm in H4. now inv H4.
+  Qed.
+  Definition before (a0 a1 : Ev) (As : tracepref) : Prop :=
+    exists n0 n1, wherein a0 As n0 /\ wherein a1 As n1 /\ n0 < n1
+  .
+  Ltac unfold_before := match goal with
+                       | [H: before _ _ _ |- _] =>
+                         let H0 := fresh "H__before" in
+                         let H1 := fresh "H__before" in
+                         unfold before in H; deex; destruct H as [H [H1 H2]]
+                       end.
+  Lemma before_nothing a0 a1 :
+    before a0 a1 nil -> False.
+  Proof.
+    intros. unfold_before; now induction n0, n1.
+  Qed.
+  Lemma before_split a As a0 a1 n :
+    a <> a0 -> a <> a1 ->
+    (before a0 a1 As) \/ (a0 = a /\ wherein a1 As n) ->
+    before a0 a1 (a :: As)
+  .
+  Proof.
+    intros Ha Hb [H1 | [H1 H2]]; try unfold_before.
+    - exists (S n0); exists (S n1); repeat split; auto. now apply Arith_prebase.lt_n_S_stt.
+    - subst; congruence.
+  Qed.
+  Lemma eat_front_in_t a b As :
+    a <> b ->
+    in_t (a) (b :: As)%list <->
+    in_t (a) (As)%list
+  .
+  Proof.
+    intros H0; split; intros [n H1].
+    - destruct n; cbn in H1.
+      + inv H1; contradiction.
+      + exists n. now inv H1.
+    - exists (S n); auto.
+  Qed.
+  Lemma eat_front_wherein a b As n :
+    a <> b ->
+    wherein a (b :: As) (S n) <->
+    wherein a As n
+  .
+  Proof.
+    intros H0; split; intros H1.
+    - now inv H1.
+    - now constructor.
+  Qed.
+  Lemma eat_front_before a b c As :
+    a <> c ->
+    b <> c ->
+    before a b (As)%list <->
+    before a b (c :: As)%list
+  .
+  Proof.
+    intros H0 H1; split; intros.
+    - unfold_before; exists (S n0). exists (S n1). repeat split.
+      now rewrite eat_front_wherein.
+      now rewrite eat_front_wherein.
+      unfold "_ < _" in *. lia.
+    - unfold_before.
+      destruct n0, n1.
+      inv H2. inv H; congruence. inv H__before0; congruence.
+      inv H; inv H__before0. exists n0; exists n1; repeat split; auto; lia.
+  Qed.
+  Lemma eat_middle_before a b c As Bs :
+    a <> c ->
+    b <> c ->
+    before a b (Bs ++ As)%list <->
+    before a b (Bs ++ c :: As)%list
+  .
+  Proof.
+  Admitted.
+  Lemma before_from_wherein a b As x x0 :
+    before (a) (b) (As)%list ->
+    wherein (a) (As)%list (x) ->
+    wherein (b) (As)%list (x0) ->
+    x < x0
+  .
+  Proof.
+    intros. unfold_before.
+    eapply wherein_eq in H, H__before0; eauto; subst; easy.
+  Qed.
+
+  Local Set Warnings "-uniform-inheritance".
+  (** Use this to define a coercion *)
+  Definition ev_to_tracepref (e : Ev) : tracepref := e :: nil.
+  Coercion ev_to_tracepref : Ev >-> tracepref.
+
+End Trace.
+
+Class PrimStep (State : Type) (Event : Type) : Type :=
+  Pstep : State -> option Event -> State -> Prop
+.
+Notation "e0 '--[' a ']-->' e1" := (Pstep e0 (Some a) e1) (at level 82, e1 at next level).
+Notation "e0 '--[,' a ']-->' e1" := (Pstep e0 a e1) (at level 82, e1 at next level).
+Notation "e0 '--[]-->' e1" := (Pstep e0 None e1) (at level 82, e1 at next level).
+
+Class EctxStep (State : Type) (Event : Type) : Type :=
+  Estep : State -> option Event -> State -> Prop
+.
+Notation "e0 '==[' a ']==>' e1" := (Estep e0 (Some a) e1) (at level 82, e1 at next level).
+Notation "e0 '==[,' a ']==>' e1" := (Estep e0 a e1) (at level 82, e1 at next level).
+Notation "e0 '==[]==>' e1" := (Estep e0 None e1) (at level 82, e1 at next level).
+
+(** Typeclass to define language with star step and all that. *)
+Class LangParams : Type := {
+  State : Type ;
+  Trace__Instance : TraceParams ;
+  step : State -> option Ev -> State -> Prop ;
+  is_value : State -> Prop ;
+}.
+
+
+Section Lang.
+  Context {langParams : LangParams}.
+  Existing Instance Trace__Instance.
+
+  Inductive star_step : State -> tracepref -> State -> Prop :=
+  | ES_refl : forall (r1 : State),
+      is_value r1 ->
+      star_step r1 nil r1
+  | ES_trans_important : forall (r1 r2 r3 : State) (a : Ev) (As : tracepref),
+      step r1 (Some a) r2 ->
+      star_step r2 As r3 ->
+      star_step r1 (a :: As) r3
+  | ES_trans_unimportant : forall (r1 r2 r3 : State) (As : tracepref),
+      step r1 None r2 ->
+      star_step r2 As r3 ->
+      star_step r1 As r3
+  .
+  Hint Constructors star_step : core.
+
+  Lemma must_step_once (S0 S2 : State) a (As : tracepref) :
+    star_step S0 (a :: As)%list S2 ->
+    exists S0' S1, step S0' (Some a) S1 /\ star_step S1 As S2
+  .
+  Proof.
+    intros H; dependent induction H; eauto.
+  Qed.
+
+  Inductive n_step : State -> nat -> tracepref -> State -> Prop :=
+  | ENS_refl : forall (r1 : State),
+      is_value r1 ->
+      n_step r1 0 nil r1
+  | ENS_trans_important : forall (r1 r2 r3 : State) (a : Ev) (As : tracepref) (n : nat),
+      step r1 (Some a) r2 ->
+      n_step r2 n As r3 ->
+      n_step r1 (S n) (a :: As) r3
+  | ENS_trans_unimportant : forall (r1 r2 r3 : State) (As : tracepref) (n : nat),
+      step r1 None r2 ->
+      n_step r2 n As r3 ->
+      n_step r1 (S n) As r3
+  .
+  Hint Constructors star_step : core.
+End Lang.
+
+Module LangNotations.
+  Context (langParams : LangParams).
+
+  Declare Scope LangNotationsScope.
+  Delimit Scope LangNotationsScope with langnotationsscope.
+  Notation "e0 '==[' a ']==>' e1" := (step e0 (Some a) e1) (at level 82, e1 at next level) : LangNotationsScope.
+  Notation "e0 '==[,' a ']==>' e1" := (step e0 a e1) (at level 82, e1 at next level) : LangNotationsScope.
+  Notation "e0 '==[]==>' e1" := (step e0 None e1) (at level 82, e1 at next level) : LangNotationsScope.
+
+  Notation "e0 '==[' a ']==>*' e1" := (star_step e0 a e1) (at level 82, e1 at next level) : LangNotationsScope.
+  Notation "e0 '==[]==>*' e1" := (star_step e0 (nil) e1) (at level 82, e1 at next level) : LangNotationsScope.
+
+  Notation "e0 '=(' n ')=[' a ']==>' e1" := (n_step e0 n a e1) (at level 82, e1 at next level) : LangNotationsScope.
+  Notation "e0 '=()=[]==>' e1" := (n_step e0 0 nil e1) (at level 82, e1 at next level) : LangNotationsScope.
+End LangNotations.
+
+#[global]
+Ltac unfold_before := match goal with
+                      | [H: before _ _ _ |- _] =>
+                        let H0 := fresh "H__before" in
+                        let H1 := fresh "H__before" in
+                        unfold before in H; deex; destruct H as [H [H1 H2]]
+                      end
+.
