coq_alt/Util/HasEquality.v
@@ -1,0 +1,81 @@
+Set Implicit Arguments.
+Require Import Setoid.
+
+Class HasEquality (A : Type) := {
+  eq : A -> A -> bool ;
+  eqb_eq : forall (a b : A), eq a b = true <-> a = b ;
+}.
+#[global]
+Infix "==" := eq (at level 81, left associativity).
+
+Lemma eq_refl { A : Type } { H : HasEquality A } (a : A) :
+  eq a a = true.
+Proof. now apply eqb_eq. Qed.
+
+Lemma eqb_dec { A : Type } { H : HasEquality A } (a x : A) :
+  eq a x = true \/ eq a x = false.
+Proof. destruct (eq a x); now (left + right). Qed.
+
+Lemma eqb_equiv_neqb { A : Type } { H : HasEquality A } (a b : A) :
+  eq a b = true <-> negb(eq a b) = negb true.
+Proof.
+  split; intros H0.
+  - rewrite H0; now cbn.
+  - destruct (eq a b); cbn in H0; auto.
+Qed.
+
+Lemma neqb_equiv_eqb { A : Type } { H : HasEquality A } (a b : A) :
+  eq a b = false <-> negb(eq a b) = negb false.
+Proof.
+  split; intros H0.
+  - rewrite H0; now cbn.
+  - destruct (eq a b); cbn in H0; auto.
+Qed.
+
+Lemma neqb_neq { A : Type } { H : HasEquality A } (a b : A) :
+  eq a b = false <-> a <> b.
+Proof.
+  split; intros H0.
+  - intros H1; subst; now rewrite eq_refl in H0.
+  - rewrite neqb_equiv_eqb; assert ((eq a b = true) -> False) by (intros H1; apply H0; now apply eqb_eq in H1);
+    destruct (eq a b); now cbn in *.
+Qed.
+Lemma eq_dec { A : Type } { H : HasEquality A } (a x : A) :
+  a = x \/ a <> x.
+Proof.
+  destruct (eqb_dec a x).
+  - apply eqb_eq in H0; now left.
+  - apply neqb_neq in H0; now right.
+Qed.
+
+#[global]
+Hint Resolve eq_refl eqb_dec eqb_equiv_neqb neqb_equiv_eqb neqb_neq eq_dec : core.
+
+Require Import CSC.Util.Convenience.
+
+Module BoolEqb.
+#[export]
+Instance eqb__Instance : HasEquality bool := {
+  eq := Bool.eqb ;
+  eqb_eq := bool_eqb_eq ;
+}.
+End BoolEqb.
+
+Ltac eq_to_defeq eq := repeat match goal with
+  | [H: context E [eq ?x ?x0] |- _] =>
+    let new := context E [(x == x0)] in
+    change new in H
+  | [ |- context E [eq ?x ?x0] ] =>
+    let new := context E [(x == x0)] in
+    change new
+  | [H: (?x == ?x0) = true |- _ ] =>
+    apply eqb_eq in H; subst
+  | [H: context E [ andb ?x ?y ] |- _] =>
+    rewrite bool_and_equiv_prop in H;
+    destruct H; subst
+  | [ |- context E [ andb ?x ?y ] ] =>
+    rewrite bool_and_equiv_prop
+  | [ |- (?x == ?x) = true ] =>
+    apply eq_refl
+  end; try easy
+.
