coq_alt/test.v
@@ -1,1 +1,0 @@
-Require Import CSC.Util. Definition i := Util.ascii_of_nat. Definition a := i.
